PoS/Invariants.v
@@ -3,7 +3,7 @@ Require Import ssreflect ssrbool ssrnat eqtype ssrfun seq.
 From mathcomp
 Require Import path.
 Require Import Eqdep pred prelude idynamic ordtype pcm finmap unionmap heap coding. 
-Require Import Blockchain Protocol Semantics.
+Require Import Blockchain Protocol Semantics States.
 Set Implicit Arguments.
 Unset Strict Implicit.
 Unset Printing Implicit Defensive.
@@ -12,12 +12,27 @@ Unset Printing Implicit Defensive.
 
 
 (* Properties *)
+(*
 Definition holds (n : nid) (w : World) (cond : State -> Prop) :=
   forall (st : State),
     find n (localState w) = Some st -> cond st.
+*)
 
 Definition has_chain (bc : Blockchain) (st : State) : Prop :=
   btChain (blockTree st) == bc.
+
+Lemma has_chain_inj :
+  forall (n : nid) (st: State) (w : World) (bc bc' : Blockchain),
+  find n (localState w) = Some st ->
+  holds n w (has_chain bc) -> holds n w (has_chain bc') -> bc = bc'.
+Proof.
+move=> n st w bc bc' sF nbc nbc'.
+rewrite /holds/has_chain in nbc nbc'.
+specialize (nbc st). specialize (nbc' st). rewrite sF in nbc nbc'.
+assert (Some st = Some st). by [].
+pose proof (nbc H) as nbc. pose proof (nbc' H) as nbc'. clear H.
+move/eqP in nbc. move/eqP in nbc'. rewrite nbc in nbc'. by [].
+Qed.
 
 Definition chain_sync_agreement (w w' : World) :=
   forall (n n' : nid) (bc bc' : Blockchain),
@@ -34,3 +49,35 @@ TODO:
 2. More complicated: the "rollback" is no more than a contstant;
 
 *)
+
+Lemma local_chain_only_grows (w w' : World) :
+  forall (n : nid) (st st' : State) (bc : Blockchain),
+    let: bc' := btChain (blockTree st') in
+    find n (localState w) = Some st ->
+    holds n w (has_chain bc) ->
+    reachable w w' ->
+    find n (localState w') = Some st' ->
+    holds n w' (has_chain bc') ->
+    size bc' <= size bc.
+Proof.
+move=> n st st' bc sF nbc R sF'.
+elim: R st st' bc nbc sF sF' => [|via z S R Hi] st st' bc nbc sF sF' nbc'.
+(* 0 steps *)
+- by pose proof (has_chain_inj sF nbc nbc'); rewrite -H; apply leqnn.
+(* Induction over system_steps *)
+- specialize (steps_nodes sF R)=>sFV.
+  specialize (gen_eta sFV). elim. move=> sv. elim. move=> svF _.
+  specialize (Hi st sv bc nbc sF svF). clear st nbc sF sFV.
+  case S. (* Prove for ONE system_step *)
+  + elim. move=> _ vzEq. rewrite vzEq in Hi svF. rewrite svF in sF'.
+    by case: sF'=>eq; rewrite eq in Hi; specialize (Hi nbc').
+  + move=> p ost _ _ _. case (procMsg ost (msg p)).
+    specialize (system_step_local_step S svF sF').
+    (* Prove for induced local transitions *)
+    move=> LS _ _ _. case LS; clear LS ost p.
+    * move=> eq. rewrite eq in svF.
+      specialize (no_change_has_held svF S nbc' sF').
+      move=> h. rewrite -eq in h. specialize (Hi h). rewrite eq in Hi.
+      by apply Hi.
+    (* TODO: Write lemmas for procMsg and procInt *)
+Qed.
